functional style

src/Distributions/DiscreteLaplace/Model.dfy
@@ -11,11 +11,41 @@ module DiscreteLaplace.Model {
   import BernoulliExpNeg
   import Bernoulli
   import Coin
+  import Loops
 
   ghost function Sample(scale: Rationals.Rational): Monad.Hurd<int>
     requires scale.numer >= 1
   {
-    SampleTailRecursive(scale)
+    var f := (x: (bool, int)) => if x.0 then -x.1 else x.1;
+    Monad.Map(SampleLoop(scale), f)
+  }
+
+  ghost function SampleLoop(scale: Rationals.Rational): Monad.Hurd<(bool, int)>
+    requires scale.numer >= 1
+  {
+    Loops.While(Condition, Body(scale))((true, 0))
+  }
+
+  ghost function Body(scale: Rationals.Rational): ((bool, int)) -> Monad.Hurd<(bool, int)>
+    requires scale.numer >= 1
+  {
+    (x: (bool, int)) => 
+      (s: Rand.Bitstream) =>
+        var (b, y) := (x.0, x.1); 
+        var (u, s) :- Uniform.Model.Sample(scale.numer)(s);
+        var (d, s) :- BernoulliExpNeg.Model.Sample(Rationals.Rational(u, scale.numer))(s);
+        if d then
+          var (v, s) :- SampleTailRecursiveHelper(scale)(s);
+          var x := u + scale.numer * v;
+          var y := x / scale.denom;
+          var (b, s) :- Coin.Model.Sample(s);
+          Monad.Result((b, y), s)
+        else 
+          Monad.Result((b, y), s)
+  }
+
+  ghost function Condition(x: (bool, int)): bool {
+    x.0 && x.1 == 0
   }
 
   ghost function SampleTailRecursive(scale: Rationals.Rational, b: bool := true, y: int := 0): Monad.Hurd<int>
@@ -33,18 +63,18 @@ module DiscreteLaplace.Model {
         else
           var (v, s) :- SampleTailRecursiveHelper(scale)(s);
           var x := u + scale.numer * v;
-          var y := x / scale.denom;
+          y := x / scale.denom;
           var sample := Coin.Model.Sample(s);
           SampleTailRecursive(scale, sample.value, y)(sample.rest)
   }
 
-  ghost function SampleTailRecursiveHelper(scale: Rationals.Rational, v: int := 0, a: bool := true): Monad.Hurd<int> {
+  ghost function SampleTailRecursiveHelper(scale: Rationals.Rational, a: bool := true, v: int := 0): Monad.Hurd<int> {
     assume {:axiom} false; // assume termination
     (s: Rand.Bitstream) =>
       if !a then
         Monad.Result(v, s)
       else
         var (a, s) :- BernoulliExpNeg.Model.Sample(Rationals.Int(1))(s);
-        SampleTailRecursiveHelper(scale, if a then v + 1 else v, a)(s)
+        SampleTailRecursiveHelper(scale, a, if a then v + 1 else v)(s)
   }
 }
