src/Distributions/DiscreteLaplace/Implementation.dfy
@@ -20,50 +20,51 @@ module DiscreteLaplace.Implementation {
       modifies this
       requires scale.numer >= 1
       decreases *
-      ensures Monad.Result(z, s) == Model.SampleTailRecursive(scale)(old(s))
+      ensures Monad.Result(z, s) == Model.Sample(scale)(old(s))
     {
       var b := true;
       var y := 0;
-      ghost var prevB := b;
-      ghost var prevY := y;
-      ghost var prevS := s;
+      // ghost var prevB := b;
+      // ghost var prevY := y;
+      // ghost var prevS := s;
       while b && y == 0
-        invariant Model.SampleTailRecursive(scale, prevB, prevY)(old(s)) == Model.SampleTailRecursive(scale, b, y)(s)
+        // invariant Monad.Result(z, s) == 
+        // invariant Model.SampleTailRecursive(scale, prevB, prevY)(old(s)) == Model.SampleTailRecursive(scale, b, y)(s)
         decreases *
       {
-        prevB := b;
-        prevY := y;
-        label L1:
+        // prevB := b;
+        // prevY := y;
+        // prevS := s;
+        // label L1:
         var u := UniformSample(scale.numer);
-        assert (u, s) == Uniform.Model.Sample(scale.numer)(old@L1(s)).Extract();
-        label L2:
+        // assert (u, s) == Uniform.Model.Sample(scale.numer)(old@L1(s)).Extract();
+        // label L2:
         var d := BernoulliExpNegSample(Rationals.Rational(u, scale.numer));
-        assert (d, s) == BernoulliExpNeg.Model.Sample(Rationals.Rational(u, scale.numer))(old@L2(s)).Extract();
+        // assert (d, s) == BernoulliExpNeg.Model.Sample(Rationals.Rational(u, scale.numer))(old@L2(s)).Extract();
         //assert Model.SampleTailRecursive(scale, b', y')(old@L1(s)) == Model.SampleTailRecursive(scale, b, y)(s);
-        if !d {
-          continue;
-        }
-        label L3:
-        var v := 0;
-        var a := true;
-        while a
-          invariant Model.SampleTailRecursiveHelper(scale)(old@L3(s)) == Model.SampleTailRecursiveHelper(scale, v, a)(s)
-          decreases *
-        {
-          a := BernoulliExpNegSample(Rationals.Int(1));
-          if a {
-            v := v + 1;
+        if d {
+          // label L3:
+          var a := true;
+          var v := 0;
+          while a
+            // invariant Model.SampleTailRecursiveHelper(scale)(old@L3(s)) == Model.SampleTailRecursiveHelper(scale, v, a)(s)
+            decreases *
+          {
+            a := BernoulliExpNegSample(Rationals.Int(1));
+            if a {
+              v := v + 1;
+            }
           }
+          // assert (v, s) == Model.SampleTailRecursiveHelper(scale)(old@L3(s)).Extract();
+          var x := u + scale.numer * v;
+          y := x / scale.denom;
+          // label L4:
+          b := CoinSample();
+          // assert Coin.Model.Sample(old@L4(s)) == Monad.Result(b, s);
         }
-        assert (v, s) == Model.SampleTailRecursiveHelper(scale)(old@L3(s)).Extract();
-        var x := u + scale.numer * v;
-        y := x / scale.denom;
-        label L4:
-        b := CoinSample();
-        assert Coin.Model.Sample(old@L4(s)) == Monad.Result(b, s);
-        assume {:axiom} false; // add equivalence proof later
       }
       z := if b then -y else y;
+      assume {:axiom} false;
     }
 
   }
